translator/ml_translatorScript.sml
@@ -1491,6 +1491,62 @@ Proof
   \\ fs [MULT_DIV]
 QED
 
+(* Encode natural-number shift counts without wrapping large shifts. *)
+Definition shift_count8_def:
+  shift_count8 sh n : word8 =
+    n2w (if sh = Ror then n MOD 8 else MIN n 8)
+End
+
+Definition shift_count64_def:
+  shift_count64 sh n : word64 =
+    n2w (if sh = Ror then n MOD 64 else MIN n 64)
+End
+
+Theorem do_arith_shift_count8[local,simp]:
+  do_arith (Shift sh) (WordT W8)
+    [Litv (Word8 w); Litv (Word8 (shift_count8 sh n))] =
+  SOME (INR (Litv (Word8 (shift8_lookup sh w n))))
+Proof
+  Cases_on `sh` >>
+  simp [shift_count8_def, do_arith_def, the_Litv_Word8_def,
+        shift8_lookup_def, dimword_def] >>
+  Cases_on `n < 8` >> simp [MIN_DEF, LSL_LIMIT, LSR_LIMIT, ASR_LIMIT] >>
+  `n MOD 8 < 256` by (
+    irule LESS_TRANS >> qexists_tac `8` >> simp []) >>
+  simp []
+QED
+
+Theorem do_arith_shift_count64[local,simp]:
+  do_arith (Shift sh) (WordT W64)
+    [Litv (Word64 w); Litv (Word64 (shift_count64 sh n))] =
+  SOME (INR (Litv (Word64 (shift64_lookup sh w n))))
+Proof
+  Cases_on `sh` >>
+  simp [shift_count64_def, do_arith_def, the_Litv_Word64_def,
+        shift64_lookup_def, dimword_def] >>
+  Cases_on `n < 64` >> simp [MIN_DEF, LSL_LIMIT, LSR_LIMIT, ASR_LIMIT] >>
+  `n MOD 64 < 2 ** 64` by (
+    irule LESS_TRANS >> qexists_tac `64` >> simp []) >>
+  fs []
+QED
+
+Theorem do_app_shift_counts[local,simp]:
+  do_app st (Arith (Shift sh) (WordT W8))
+    [Litv (Word8 w8); Litv (Word8 (shift_count8 sh n))] =
+    SOME (st, Rval (Litv (Word8 (shift8_lookup sh w8 n)))) /\
+  do_app st (Arith (Shift sh) (WordT W64))
+    [Litv (Word64 w64); Litv (Word64 (shift_count64 sh n))] =
+    SOME (st, Rval (Litv (Word64 (shift64_lookup sh w64 n))))
+Proof
+  Cases_on `st` >> simp [do_app_def, check_type_def]
+QED
+
+Overload ShiftExp[local] =
+  ``\sz sh n x.
+      App (Arith (Shift sh) (WordT sz))
+        [x; Lit (if sz = W8 then Word8 (shift_count8 sh n)
+                 else Word64 (shift_count64 sh n))]``;
+
 Theorem Eval_w2n:
     Eval env x1 (WORD (w:'a word)) ==>
     Eval env
@@ -1499,9 +1555,9 @@ Theorem Eval_w2n:
        else if dimindex (:'a) = 64 then
          App (FromTo (WordT W64) IntT) [x1]
        else if dimindex (:'a) < 8 then
-         App (FromTo (WordT W8) IntT) [App (Shift W8 Lsr (8 - dimindex (:'a))) [x1]]
+         App (FromTo (WordT W8) IntT) [ShiftExp W8 Lsr (8 - dimindex (:'a)) x1]
        else
-         App (FromTo (WordT W64) IntT) [App (Shift W64 Lsr (64 - dimindex (:'a))) [x1]])
+         App (FromTo (WordT W64) IntT) [ShiftExp W64 Lsr (64 - dimindex (:'a)) x1])
       (NUM (w2n w))
 Proof
   rw[Eval_rw,WORD_def] \\ fs []
@@ -1551,9 +1607,9 @@ Theorem Eval_i2w:
        else if dimindex (:'a) = 64 then
          App (FromTo IntT (WordT W64)) [x1]
        else if dimindex (:'a) < 8 then
-         App (Shift W8 Lsl (8 - dimindex (:'a))) [App (FromTo IntT (WordT W8)) [x1]]
+         ShiftExp W8 Lsl (8 - dimindex (:'a)) (App (FromTo IntT (WordT W8)) [x1])
        else
-         App (Shift W64 Lsl (64 - dimindex (:'a))) [App (FromTo IntT (WordT W64)) [x1]])
+         ShiftExp W64 Lsl (64 - dimindex (:'a)) (App (FromTo IntT (WordT W64)) [x1]))
       (WORD ((i2w n):'a word))
 Proof
   rw[Eval_rw,WORD_def] \\ fs [] \\ rfs []
@@ -1592,12 +1648,13 @@ Theorem Eval_n2w:
        else if dimindex (:'a) = 64 then
          App (FromTo IntT (WordT W64)) [x1]
        else if dimindex (:'a) < 8 then
-         App (Shift W8 Lsl (8 - dimindex (:'a))) [App (FromTo IntT (WordT W8)) [x1]]
+         ShiftExp W8 Lsl (8 - dimindex (:'a)) (App (FromTo IntT (WordT W8)) [x1])
        else
-         App (Shift W64 Lsl (64 - dimindex (:'a))) [App (FromTo IntT (WordT W64)) [x1]])
+         ShiftExp W64 Lsl (64 - dimindex (:'a)) (App (FromTo IntT (WordT W64)) [x1]))
       (WORD ((n2w n):'a word))
 Proof
-  qsuff_tac `n2w n = i2w (& n)` THEN1 fs [Eval_i2w,NUM_def]
+  qsuff_tac `(n2w n : 'a word) = i2w (& n)` THEN1
+    fs [SIMP_RULE (srw_ss()) [] Eval_i2w, NUM_def]
   \\ fs [integer_wordTheory.i2w_def]
 QED
 
@@ -1608,17 +1665,17 @@ Theorem Eval_w2w:
       (if (dimindex (:'a) <= 8 <=> dimindex (:'b) <= 8) then
          let w = if dimindex (:'a) <= 8 then W8 else W64 in
            if dimindex (:'b) <= dimindex (:'a) then
-             App (Shift w Lsr (dimindex (:'a) - dimindex (:'b))) [x1]
+             ShiftExp w Lsr (dimindex (:'a) - dimindex (:'b)) x1
            else
-             App (Shift w Lsl (dimindex (:'b) - dimindex (:'a))) [x1]
+             ShiftExp w Lsl (dimindex (:'b) - dimindex (:'a)) x1
        else if dimindex (:'b) <= 8 then
-         App (Shift W64 Lsl (64 - dimindex (:'a)))
-           [App (Shift W64 Lsr (8 - dimindex (:'b)))
-              [App (FromTo IntT (WordT W64)) [App (FromTo (WordT W8) IntT) [x1]]]]
+         ShiftExp W64 Lsl (64 - dimindex (:'a))
+           (ShiftExp W64 Lsr (8 - dimindex (:'b))
+             (App (FromTo IntT (WordT W64)) [App (FromTo (WordT W8) IntT) [x1]]))
        else
-         App (Shift W8 Lsl (8 - dimindex (:'a)))
-           [App (FromTo IntT (WordT W8)) [App (FromTo (WordT W64) IntT)
-              [App (Shift W64 Lsr (64 - dimindex (:'b))) [x1]]]])
+         ShiftExp W8 Lsl (8 - dimindex (:'a))
+           (App (FromTo IntT (WordT W8)) [App (FromTo (WordT W64) IntT)
+              [ShiftExp W64 Lsr (64 - dimindex (:'b)) x1]]))
       (WORD ((w2w w):'a word))
 Proof
   IF_CASES_TAC THEN1
@@ -1664,12 +1721,12 @@ QED
 Theorem Eval_word_lsl:
    !n.
       Eval env x1 (WORD (w1:'a word)) ==>
-      Eval env (App (Shift (if dimindex (:'a) <= 8 then W8 else W64) Lsl n) [x1])
+      Eval env (ShiftExp (if dimindex (:'a) <= 8 then W8 else W64) Lsl n x1)
         (WORD (word_lsl w1 n))
 Proof
-  rw[Eval_rw,WORD_def]
+  rw[Eval_rw,WORD_def] \\ fs []
   \\ pop_assum (qspec_then `refs` mp_tac) \\ strip_tac
-  \\ qexists_tac `ck1` \\ fs [do_app_def,empty_state_def]
+  \\ qexists_tac `ck1` \\ fs [do_app_def,empty_state_def,check_type_def]
   \\ fs [LESS_EQ_EXISTS]
   \\ qpat_x_assum ‘_ + _ = NUMERAL _’ (assume_tac o GSYM)
   \\ full_simp_tac std_ss []
@@ -1684,14 +1741,14 @@ Theorem Eval_word_lsr:
       Eval env (let w = (if dimindex (:'a) <= 8 then W8 else W64) in
                 let k = (if dimindex (:'a) <= 8 then 8 else 64) - dimindex(:'a) in
                   if dimindex (:'a) = 8 \/ dimindex (:'a) = 64 then
-                    App (Shift w Lsr n) [x1]
+                    ShiftExp w Lsr n x1
                   else
-                    App (Shift w Lsl k) [App (Shift w Lsr (n+k)) [x1]])
+                    ShiftExp w Lsl k (ShiftExp w Lsr (n+k) x1))
         (WORD (word_lsr w1 n))
 Proof
   rw[Eval_rw,WORD_def]
   \\ first_x_assum (qspec_then `refs` mp_tac) \\ strip_tac
-  \\ qexists_tac `ck1` \\ fs [do_app_def,empty_state_def]
+  \\ qexists_tac `ck1` \\ fs [do_app_def,empty_state_def,check_type_def]
   \\ TRY
    (fs [do_app_def,shift8_lookup_def,shift64_lookup_def]
     \\ fs [fcpTheory.CART_EQ,word_lsr_def,fcpTheory.FCP_BETA,w2w] \\ rw []
@@ -1713,14 +1770,14 @@ Theorem Eval_word_asr:
       Eval env (let w = (if dimindex (:'a) <= 8 then W8 else W64) in
                 let k = (if dimindex (:'a) <= 8 then 8 else 64) - dimindex(:'a) in
                   if dimindex (:'a) = 8 \/ dimindex (:'a) = 64 then
-                    App (Shift w Asr n) [x1]
+                    ShiftExp w Asr n x1
                   else
-                    App (Shift w Lsl k) [App (Shift w Asr (n+k)) [x1]])
+                    ShiftExp w Lsl k (ShiftExp w Asr (n+k) x1))
         (WORD (word_asr w1 n))
 Proof
   rw[Eval_rw,WORD_def]
   \\ first_x_assum (qspec_then `refs` mp_tac) \\ strip_tac
-  \\ qexists_tac `ck1` \\ fs [do_app_def,empty_state_def]
+  \\ qexists_tac `ck1` \\ fs [do_app_def,empty_state_def,check_type_def]
   \\ TRY (* takes care of = 8 and = 64 cases *)
    (fs [do_app_def,shift8_lookup_def,shift64_lookup_def]
     \\ fs [fcpTheory.CART_EQ,word_asr_def,fcpTheory.FCP_BETA,w2w] \\ rw []
@@ -1742,14 +1799,14 @@ Theorem Eval_word_ror:
    !n.
       Eval env x1 (WORD (w1:'a word)) ==>
       (dimindex (:'a) <> 8 ==> dimindex (:'a) = 64) ==>
-      Eval env (App (Shift (if dimindex (:'a) <= 8 then W8 else W64) Ror n) [x1])
+      Eval env (ShiftExp (if dimindex (:'a) <= 8 then W8 else W64) Ror n x1)
         (WORD (word_ror w1 n))
 Proof
   Cases_on `dimindex (:'a) = 8` \\ fs []
   \\ Cases_on `dimindex (:'a) = 64` \\ fs []
   \\ rw[Eval_rw,WORD_def]
   \\ first_x_assum (qspec_then `refs` mp_tac) \\ strip_tac
-  \\ qexists_tac `ck1` \\ fs [do_app_def,empty_state_def]
+  \\ qexists_tac `ck1` \\ fs [do_app_def,empty_state_def,check_type_def]
   \\ fs [LESS_EQ_EXISTS]
   \\ fs [do_app_def,shift8_lookup_def,shift64_lookup_def]
   \\ fs [fcpTheory.CART_EQ,word_ror_def,fcpTheory.FCP_BETA,w2w] \\ rw []
